clean chi soundness proof

Clean/Gadgets/Keccak/Chi.lean
@@ -12,13 +12,11 @@ open Gadgets.Keccak256 (KeccakState)
 open Bitwise (not64)
 open Not (not64_bytewise not64_bytewise_value)
 
-def xor (x y : Var U64 (F p)) := subcircuit Xor.circuit ⟨x, y⟩
-def and (x y : Var U64 (F p)) := subcircuit And.And64.circuit ⟨x, y⟩
-def not (x : Var U64 (F p)) := subcircuit Not.circuit x
-
 def main (state : Var KeccakState (F p)) : Circuit (F p) (Var KeccakState (F p)) :=
   Vector.finRange 25 |>.mapM fun i => do
-    xor (state.get i) (←and (←not (state.get (i + 5))) (state.get (i + 10)))
+    let state_not ← subcircuit Not.circuit (state.get (i + 5))
+    let state_and ← subcircuit And.And64.circuit ⟨state_not, state.get (i + 10)⟩
+    subcircuit Xor.circuit ⟨state.get i, state_and⟩
 
 def assumptions := KeccakState.is_normalized (p:=p)
 
@@ -26,16 +24,8 @@ def spec (state : KeccakState (F p)) (out_state : KeccakState (F p)) :=
   out_state.is_normalized
   ∧ out_state.value = Specs.Keccak256.chi state.value
 
-instance lawfulBody (state : Var KeccakState (F p)) : ConstantLawfulCircuits (fun i => do
-  xor (state.get i) (←and (←not (state.get (i + 5))) (state.get (i + 10)))
-) := ConstantLawfulCircuits.from_constant_length
-  (by dsimp only [xor, not, and]; infer_lawful_circuit)
-  (by intros; ac_rfl)
-
-instance lawful (state : Var KeccakState (F p)) : LawfulCircuit (main state) := .from_mapM_vector _ (by
-  have := ConstantLawfulCircuits.to_single (lawful := lawfulBody state)
-  infer_instance
-)
+instance lawful (state : Var KeccakState (F p)) : ConstantLawfulCircuit (main state) :=
+  .from_mapM_vector _ (by infer_constant_lawful_circuits)
 
 -- #eval! main (p:=p_babybear) default |>.operations.local_length
 -- #eval! main (p:=p_babybear) default |>.output
@@ -43,76 +33,71 @@ instance elaborated : ElaboratedCircuit (F p) KeccakState (Var KeccakState (F p)
   main
   local_length _ := 400
   local_length_eq state i0 := by
-    rw [main, Circuit.mapM_vector_local_length]
-    dsimp only [lawful_norm, circuit_norm, lawfulBody, Not.circuit, And.And64.circuit, Xor.circuit]
+    rw [LawfulCircuit.local_length_eq]
+    simp only [lawful_norm, Not.circuit, And.And64.circuit, Xor.circuit]
 
   initial_offset_eq state i := LawfulCircuit.initial_offset_eq (main state) i
 
-  output _ i0 := #v[
-    var_from_offset U64 (i0 + 8),
-    var_from_offset U64 (i0 + 24),
-    var_from_offset U64 (i0 + 40),
-    var_from_offset U64 (i0 + 56),
-    var_from_offset U64 (i0 + 72),
-    var_from_offset U64 (i0 + 88),
-    var_from_offset U64 (i0 + 104),
-    var_from_offset U64 (i0 + 120),
-    var_from_offset U64 (i0 + 136),
-    var_from_offset U64 (i0 + 152),
-    var_from_offset U64 (i0 + 168),
-    var_from_offset U64 (i0 + 184),
-    var_from_offset U64 (i0 + 200),
-    var_from_offset U64 (i0 + 216),
-    var_from_offset U64 (i0 + 232),
-    var_from_offset U64 (i0 + 248),
-    var_from_offset U64 (i0 + 264),
-    var_from_offset U64 (i0 + 280),
-    var_from_offset U64 (i0 + 296),
-    var_from_offset U64 (i0 + 312),
-    var_from_offset U64 (i0 + 328),
-    var_from_offset U64 (i0 + 344),
-    var_from_offset U64 (i0 + 360),
-    var_from_offset U64 (i0 + 376),
-    var_from_offset U64 (i0 + 392)
-  ]
+  output _ i0 :=  Vector.natInit 25 fun i => var_from_offset U64 (i0 + i*16 + 8)
   output_eq state i := by
-    dsimp only [circuit_norm, main]
-    -- TODO need theorem about output of `mapM`!
-    sorry
+    rw [LawfulCircuit.output_eq]
+    simp only [lawful_norm, lawful, Xor.circuit, And.And64.circuit, Not.circuit]
+    simp [Vector.finRange, List.finRange, Vector.range_succ, Array.range]
+
+-- rewrite the chi spec as a loop
+lemma chi_loop (state : Vector ℕ 25) :
+    Specs.Keccak256.chi state = .init fun i => state[i] ^^^ ((not64 state[i + 5]) &&& state[i + 10]) := by
+  rw [Specs.Keccak256.chi, Vector.init, Vector.finRange, Vector.map_mk, Vector.eq_mk, List.map_toArray]
+  rfl
 
 theorem soundness : Soundness (F p) assumptions spec := by
-  intro i env state_var state h_input state_norm h_holds
+  intro i0 env state_var state h_input state_norm h_holds
 
-  have h_input' (i : Fin 25) : eval env state_var[i.val] = state[i.val] := by
-    rw [←h_input, eval_vector, Vector.getElem_map]
-
-  have h_input_not (i : Fin 25) : (eval env (not64_bytewise state_var[i.val])) = not64_bytewise_value state[i.val] := by
-    rw [←h_input', Not.eval_not]
-
-  have h_not_value (i : Fin 25) : (not64_bytewise_value state[i.val]).value = not64 state[i.val].value :=
-    (Not.not_bytewise_value_spec (state_norm i)).left
-
-  have h_not_normalized (i : Fin 25) : (not64_bytewise_value state[i.val]).is_normalized :=
-    (Not.not_bytewise_value_spec (state_norm i)).right
-
-  simp only [circuit_norm, spec, KeccakState.is_normalized_iff,
-    Specs.Keccak256.chi, KeccakState.value, eval_vector,
-    Array.mk.injEq, List.cons.injEq, and_true]
   simp only [assumptions, KeccakState.is_normalized, Fin.getElem_fin] at state_norm
 
-  dsimp only [circuit_norm, main,
-    not, xor, and, Xor.circuit, And.And64.circuit, Not.circuit] at h_holds
-  simp only [circuit_norm, subcircuit_norm, Xor.assumptions, Xor.spec,
-    And.And64.assumptions, And.And64.spec] at h_holds
+  -- simplify goal
+  simp only [spec, lawful_norm]
+  rw [chi_loop, eval_vector, KeccakState.is_normalized, Vector.ext_iff]
+  simp only [Fin.getElem_fin, Vector.getElem_map, Vector.getElem_natInit, Vector.getElem_init,
+    KeccakState.value, Vector.map_map, Function.comp_apply]
 
-  simp only [h_input', h_input_not, h_not_value, state_norm, h_not_normalized,
-    and_self, imp_self, forall_const, true_and, and_imp, and_assoc, and_true] at h_holds
+  suffices h : ∀ i : Fin 25, (eval env (var_from_offset U64 (i0 + i.val*16 + 8))).is_normalized ∧
+    (eval env (var_from_offset U64 (i0 + i.val*16 + 8))).value =
+      state.value[i] ^^^ ((not64 state.value[i + 5]) &&& state.value[i + 10]) by
+    constructor
+    · intro i; exact (h i).left
+    · intro i' hi'
+      specialize h ⟨ i', hi'⟩
+      simp_all [KeccakState.value]
 
-  simp_all [not64, Specs.Keccak256.not_u64]
-  and_intros <;> rfl
+  -- simplify constraints using mapM theory
+  simp only [elaborated, main] at h_holds
+  rw [Circuit.constraints_hold.mapM_vector_soundness (lawful := by infer_constant_lawful_circuits)] at h_holds
+  simp only [circuit_norm, lawful_norm, subcircuit_norm, Xor.circuit, And.And64.circuit, Not.circuit,
+    Xor.assumptions, Xor.spec, And.And64.assumptions, And.And64.spec, Nat.reduceAdd] at h_holds
+
+  -- TODO: this would be simpler if we had special theorems about Vector.finRange loops
+  intro i
+  specialize h_holds i
+  have : i ∈ Vector.finRange 25 := by simp [Vector.finRange]
+  specialize h_holds this i
+  have : (i, ↑i) ∈ (Vector.finRange 25).zipIdx := by
+    simp only [Vector.mem_zipIdx_iff_getElem?, Fin.is_lt, Vector.getElem?_eq_getElem, Option.some.injEq]
+    simp [Vector.finRange]
+  specialize h_holds this
+
+  have h_input (i : Fin 25) : eval env state_var[i.val] = state[i.val] := by
+    rw [←h_input, eval_vector, Vector.getElem_map]
+
+  have h_input_not : (eval env (not64_bytewise state_var[(i + 5).val])) = not64_bytewise_value state[((i + 5)).val] := by
+    rw [←h_input, Not.eval_not]
+
+  have ⟨ state_not_value, state_not_norm ⟩ := Not.not_bytewise_value_spec (state_norm (i + 5))
+  simp_all [KeccakState.value]
 
 theorem completeness : Completeness (F p) KeccakState assumptions := by
   intro i env state_var h_env state h_input state_norm
+  stop
 
   have h_input' (i : Fin 25) : eval env state_var[i.val] = state[i.val] := by
     rw [←h_input, eval_vector, Vector.getElem_map]
